#+TITLE: How to prove the arithmetic mean and geometric mean formula
#+DATE: <2019-08-31 åœŸ>
#+AUTHOR: hisanobu-nakamura
#+EMAIL: 369bodhisattva@gmail
#+OPTIONS: ':nil *:t -:t ::t <:t H:3 \n:nil ^:t arch:headline
#+OPTIONS: author:t c:nil creator:comment d:(not "LOGBOOK") date:t
#+OPTIONS: e:t email:nil f:t inline:t num:t p:nil pri:nil stat:t
#+OPTIONS: tags:t tasks:t tex:t timestamp:t toc:t todo:t |:t
#+CREATOR: Emacs 25.3.2 (Org mode 8.2.10)
#+DESCRIPTION:
#+EXCLUDE_TAGS: noexport
#+KEYWORDS:
#+LANGUAGE: en
#+SELECT_TAGS: export
#+LATEX_HEADER: \usepackage[margin=1.0in]{geometry}
#+LATEX_HEADER: \usepackage{mymacros}


\begin{equation*}
\label{ }
\frac{a_1 + \cdots + a_n}{n} \ge \sqrt[n]{a_1\cdots a_n}
\end{equation*}
where $\forall i \; a_i > 0$ \\
\begin{proof}
OK for n=1. Equality holds. Suppose that the inequality holds for all natural numbers up to n, then
\begin{eqnarray*}
a_1 + \cdots + a_{n+1} & = & \frac{a_2 + a_3 \cdots + a_{n+1}}{n} + \frac{a_1 + a_3 + \cdots + a_{n+1}}{n} + \cdots  \nonumber \\
 &  &  + \frac{a_1 + a_2 + \overset{i}{\breve{\cdots} } + a_{n+1}}{n} + \cdots + \frac{a_1 + \cdots + a_{n}}{n}\nonumber\\
 & = &  \sqrt[n]{a_2\cdots a_{n+1}} + \cdots + \sqrt[n]{a_1\cdots a_n} \nonumber \\
  & = &  \sqrt[n+1]{a_1\cdots a_{n+1}} \left( \frac{\sqrt[n]{a_2\cdots a_{n+1}}}{\sqrt[n+1]{a_1\cdots a_{n+1}}} + \cdots + \frac{\sqrt[n]{a_1\cdots a_n}}{\sqrt[n+1]{a_1\cdots a_{n+1}}} \right) \nonumber \\
   & = &  \sqrt[n+1]{a_1\cdots a_{n+1}} \left( \sqrt[n+1]{\frac{\sqrt[n]{a_2\cdots a_{n+1}}}{a_1}} + \cdots + \sqrt[n+1]{\frac{\sqrt[n]{a_1\cdots a_{n}}}{a_{n+1}}}\right) \nonumber \\
   & = &  \sqrt[n+1]{a_1\cdots a_{n+1}} \left( \sqrt[n+1]{\frac{\alpha_1}{a_1}} + \cdots + \sqrt[n+1]{\frac{\alpha_{n+1}}{a_{n+1}}}\right) 
\end{eqnarray*}
where $\alpha_i = \sqrt[n]{a_1\overset{i}{\breve{\cdots} } a_{n+1}}$ \; (Here, $\overset{i}{\breve{\cdots} }$ means omitting the i-th term in the sum or the product). It is easy to see that 
\begin{equation*}
\label{ }
\sqrt[n+1]{\frac{\alpha_1}{a_1}}  \cdots  \sqrt[n+1]{\frac{\alpha_{n+1}}{a_{n+1}}} = 1.
\end{equation*}
So, if we can show the following proposition, we are done.
\begin{prop_non}
 If $b_1, \cdots, b_{n+1} >0$, $\forall i \;b_i \ne 1$ and $b_1 \cdots b_{n+1} = 1$, then
\begin{equation}
\label{AM_GM_normalised}
b_1 + \cdots + b_{n+1} \ge n+1
\end{equation}
\end{prop_non}
\begin{proof}
 Let us prove by induction, but before we begin the proof, notice that among $b_i$s there exist at least one number that is larger or smaller than $1$ respectively. \\
So, for $n=1$, we can assume that $b_1 = 1-c_1$ with $0 < c_1 <1$. Then
\begin{equation*}
\label{ }
b_1 + b_2 = b_1 + \frac{1}{b_1} = 1 - c_1 + \frac{1}{1-c_1} \ge 1-c_1 + 1 + c_1 = 2.
\end{equation*}
Now, let us suppose that (\ref{AM_GM_normalised}) holds true for all the natural numbers up to n. Regarding the fact mentioned above, let us suppose that $b_n = 1 + c_n$ and $b_{n+1} = 1+c_{n+1}$ with $c_n < 0$ and $c_{n+1} > 0$. Then, by the assumption, 
\begin{equation*}
\label{ }
(b_1 \cdots b_{n-1})(b_n b_{n+1}) = 1 \implies b_1 + \cdots + b_{n-1} + b_n b_{n+1} \ge n.
\end{equation*}
If we can say
\begin{equation*}
\label{ }
b_1 + \cdots + b_{n-1} + (b_n + b_{n+1}) \ge b_1 + \cdots b_{n-1} + (b_n b_{n+1} + 1),
\end{equation*}
then the inequality follows. But
\begin{equation*}
\label{ }
b_n + b_{n+1} - (b_n b_{n+1} + 1) = -c_n c_{n+1} > 0.
\end{equation*}
Hence, it follows that 
\begin{equation*}
\label{ }
b_1 + \cdots + b_{n-1} + b_n + b_{n+1} \ge b_1 + \cdots + b_{n-1} + b_n b_{n+1} + 1 \ge n + 1
\end{equation*}
\end{proof}
Now, by substituting $b_i = \sqrt[n+1]{\frac{\alpha_i}{a_i}}$, it is straightforward to see that
\begin{eqnarray*}
a_1 + \cdots + a_{n+1} & = &  \sqrt[n+1]{a_1\cdots a_{n+1}} \left( \sqrt[n+1]{\frac{\alpha_1}{a_1}} + \cdots + \sqrt[n+1]{\frac{\alpha_{n+1}}{a_{n+1}}}\right) \nonumber \\
					   & \ge &  \sqrt[n+1]{a_1\cdots a_{n+1}} (n + 1 ) \nonumber \\
\end{eqnarray*}
\end{proof}

