% Created 2021-07-01 木 11:56
% Intended LaTeX compiler: pdflatex
\documentclass{article}
\usepackage[utf8]{inputenc}
\usepackage[T1]{fontenc}
\usepackage{graphicx}
\usepackage{grffile}
\usepackage{longtable}
\usepackage{wrapfig}
\usepackage{rotating}
\usepackage[normalem]{ulem}
\usepackage{amsmath}
\usepackage{textcomp}
\usepackage{amssymb}
\usepackage{capt-of}
\usepackage{hyperref}
\date{\textit{<2021-07-01 木>}}
\title{Reflections of Pinor group representations}
\hypersetup{
 pdfauthor={},
 pdftitle={Reflections of Pinor group representations},
 pdfkeywords={},
 pdfsubject={},
 pdfcreator={Emacs 27.2 (Org mode 9.4.4)}, 
 pdflang={English}}
\begin{document}

\maketitle
Title: Reflections of Pinor group representations
Date: 2021-07-01
Category: math
Tags: math, Clifford-Algebra

\section{Clifford Algebra and Pinor group}
\label{sec:orgbc9cbe9}

Let \(\text{Cl}(N)\) be a Clifford algebra of dimension \(N\), and \(e_{i} \in \text{Cl}(N),\; i=1,...,N\) be a orthogonal basis. 
Let us consider a unit vector \(n = \sum_{i=1}^{N} n_{i}e_{i}\) with \(||n||=1\) and its action on a vector \(x = \sum_{i=1}^{N} x_{i}e_{i}\) determined by the Pinor representation \(\alpha: Pin(N) \rightarrow O(N)\):
\begin{equation*}
\alpha(n)(x) := nx^tn.
\end{equation}
Let's calculate the explicit expression of this action!
\begin{eqnarray}
\alpha(n)(x) & = & \sum_{i,j,k=1}^{N} n_{i}x_{j}n_{k}e_{i}e_{j}e_{k}\nonumber\\ 
& = & \sum_{i} n_{i}x_{i}n_{i}e_{i}e_{i}e_{i} + \sum_{i \ne j} n_{i}x_{i}n_{j}e_{i}e_{i}e_{j} + \sum_{i \ne j} n_{i}x_{j}n_{i}e_{i}e_{j}e_{i} + \sum_{i \ne j} n_{j}x_{i}n_{i}e_{j}e_{i}e_{i} + \sum_{i \ne j \ne k} n_{i}x_{j}n_{k}e_{i}e_{j}e_{k} \nonumber \\
& = & -\sum_{i} n_{i}x_{i}n_{i}e_{i} - \sum_{i \ne j} n_{i}x_{i}n_{j}e_{j} + \sum_{i \ne j} n_{i}x_{j}n_{i}e_{j} - \sum_{i \ne j} n_{j}x_{i}n_{i}e_{j} + \sum_{i \ne j \ne k} n_{i}x_{j}n_{k}e_{i}e_{j}e_{k} \nonumber \\
& = &  - \sum_{i, j=1}^{N} n_{i}x_{i}n_{j}e_{j} + \sum_{i, j=1}^{N} n_{i}x_{j}n_{i}e_{j} - \sum_{i, j}^{N} n_{j}x_{i}n_{i}e_{j} + \sum_{i \ne j \ne k} n_{i}x_{j}n_{k}e_{i}e_{j}e_{k} \nonumber \\
& = & \sum_{i=1}^{N} x_{i}e_{i} - 2 \sum_{i, j}^{N} n_{i}x_{i}n_{j}e_{j} + \sum_{i \ne j \ne k} n_{i}x_{j}n_{k}e_{i}e_{j}e_{k}
\end{eqnarray}
The last term is zero, because
\begin{equation}
 \sum_{i \ne j \ne k} n_{i}x_{j}n_{k}e_{i}e_{j}e_{k} =  -\sum_{i \ne j \ne k} n_{i}x_{j}n_{k}e_{k}e_{j}e_{i} =  -\sum_{i \ne j \ne k} n_{i}x_{j}n_{k}e_{i}e_{j}e_{k}
\end{equation}
Hence,
\begin{equation}
\alpha(n)(x) = \sum_{i=1}^{N} x_{i}e_{i} - 2 \sum_{i, j=1}^{N} n_{i}x_{i}n_{j}e_{j} = x - 2 (n,x)n
\end{equation}
, which is a reflection in \(n\).
\end{document}