#+TITLE: Elliptic and Theta Functions
#+DATE: <2019-08-31 土>
#+AUTHOR: hisanobu-nakamura
#+EMAIL: 369bodhisattva@gmail
#+OPTIONS: ':nil *:t -:t ::t <:t H:3 \n:nil ^:t arch:headline
#+OPTIONS: author:t c:nil creator:comment d:(not "LOGBOOK") date:t
#+OPTIONS: e:t email:nil f:t inline:t num:t p:nil pri:nil stat:t
#+OPTIONS: tags:t tasks:t tex:t timestamp:t toc:t todo:t |:t
#+CREATOR: Emacs 25.3.2 (Org mode 8.2.10)
#+DESCRIPTION:
#+EXCLUDE_TAGS: noexport
#+KEYWORDS:
#+LANGUAGE: en
#+SELECT_TAGS: export

* About this note
This note contains notes for Kotan seminar on elliptic and theta functions.

* Examples of Elliptic Integrals
Here, we gather some examples varying from pure mathematics to physics
** Arc Length of Ellipse
Canonical form (標準形):
\begin{equation}
\frac{x^{2}}{a^{2}} +\frac{y^{2}}{b^{2}}=1 \quad with \; a \ge b.
\end{equation}
 
Parametric form
\begin{equation}
\mathbf{p} =\left(
\begin{array}{c}
 x \\
 y
\end{array} \right)
=\left(
\begin{array}{c}
 a \sin{\varphi} \\
 b \cos{\varphi}
\end{array} \right)
\;, where \; 0 \le \varphi < 2 \pi
\end{equation}
The length of a curve $\mathbf{p}(t) = (x(t), y(t))$ is
\begin{eqnarray}
s(u) &=& \int_{0}^{u} \left| \frac{d \mathbf{p}}{d t} \right| dt  \\ \nonumber
     &=& \int_{0}^{u} \sqrt{ \left( \frac{d x}{d t} \right)^{2} +  \left( \frac{d x}{d t} \right)^{2} } \; dt
\end{eqnarray}
For the ellipse's case, we have
\begin{eqnarray}
s(\varphi) &=& \int_{0}^{\varphi} \sqrt{ a^{2} \cos^{2}{\varphi} +  b^{2}  \sin^{2}{\varphi}} \; d\varphi \\ \nonumber
     &=& a \int_{0}^{u} \sqrt{ 1 -  k^{2}  \sin^{2}{\varphi}} \; d\varphi 
\end{eqnarray}
where we defined $k = \sqrt{\frac{a^2 - b^2}{a^2}}$.
\begin{eqnarray}
E(k, \varphi ) &:=& \int_{0}^{u} \sqrt{ 1 -  k^{2}  \sin^{2}{\varphi}} \; d\varphi \\
E(k) &:=& E(k,  \pi/2 )
\end{eqnarray}
$E(k, \varphi )$ is called the *second incomplete elliptic integral (第2種不完全楕円積分)* and $E(k)$ the *second complete elliptic integral (第2種完全楕円積分)*. The total length $s_{total}$ of the ellipse is given by 
\begin{equation}
s_{total} = 4a E(k) 
\end{equation}
Alternatively, putting $y = \pm b \sqrt{1 - \frac{x^{2}}{a^{2}}}, the length can also be obtained as
\begin{eqnarray}
s &=& \int_{0}^{x} \sqrt{ 1  +  \left( \frac{d x}{d t} \right)^{2} } \; dx \\ \nonumber
     &=& a \int_{0}^{x} \sqrt{ 1  +   \frac{b^{2}}{a^{2}} \frac{\frac{x^{2}}{a^{2}}}{1 - \frac{x^{2}}{a^{2}}} } \; dx
\end{eqnarray}
Let us substitute further with $z = \frac{x}{a}$, we have
| $x$ | $0 \rightarrow a$ |
|-----+-------------------|
| $z$ | $0 \rightarrow 1$ |

\begin{eqnarray}
s &=& a \int_{0}^{z} \sqrt{ 1  +   \frac{b^{2}}{a^{2}} \frac{z^{2}}{1 - z^{2}} } \; dx \\ \nonumber
  &=& a \int_{0}^{z} \sqrt{ \frac{1 -k ^{2} z^{2}}{1 - z^{2}} } \; dx.
\end{eqnarray}
